Work in progress for Aligned decode string with term string and some progress on the remaining holes for CorrectDecoder for decode string with term string.

src/Narcissus/BinLib/WithTerm/String.v
@@ -10,6 +10,8 @@ Require Import
         Fiat.Narcissus.BinLib.AlignedEncodeMonad
         Fiat.Narcissus.BinLib.AlignedDecodeMonad
         Fiat.Narcissus.BinLib.AlignedString.
+Require Import Recdef.
+Require Import Operations.
 
 Section String.
   Context {cache : Cache}.
@@ -25,10 +27,867 @@ Section String.
 
   Open Scope AlignedDecodeM_scope.
 
-  Definition AlignedDecodeStringWithTerm {m}
+(* GetByteAt *)
+(*   Fixpoint StringTermAlignedDecodeM {m} *)
+(*            (term_char : word 8) *)
+(*            (n : nat) *)
+(*     : AlignedDecodeM string m := *)
+(*     match n with *)
+(*     | 0 => ThrowAlignedDecodeM *)
+(*     | S n' => BindAlignedDecodeM GetCurrentByte *)
+(*           (fun c => if (weqb c term_char) *)
+(*                      then ReturnAlignedDecodeM EmptyString *)
+(*                    else BindAlignedDecodeM (StringTermAlignedDecodeM term_char n') *)
+(*                      (fun s => ReturnAlignedDecodeM (String (ascii_of_N (wordToN c)) s))) *)
+(*     end%AlignedDecodeM%list. *)
+
+  (* Want to use auto to solve the termination condition *) 
+  Local Hint Extern 4 =>
+  match goal with
+  | H : Nat.leb _ _ = false  |- _ => 
+    apply Compare_dec.leb_complete_conv in H; lia
+  | H : {res : nat & _ = S _} |- _ =>
+    destruct H; simpl; red; auto
+  end.
+  
+  Declare Scope option.
+  Notation "res <- c ; k" := (option_bind (fun res => k) c) : option.
+  Require Import Bedrock.Word Ascii.
+
+  Open Scope string.
+  Open Scope option.
+
+  Fixpoint sequence (l : list (option Core.char)) : option string :=
+    match l with
+    | nil => Some ""
+    | h::t => 
+      h' <- h;
+      rec <- sequence t;
+      Some (String (ascii_of_N (wordToN h')) rec)
+  end.
+  Definition GetCurrentByte_dep 
+             {n : nat}
+             (v: ByteBuffer.t n)
+             (idx : nat) : CacheDecode -> option (Core.char * {res : nat & res = S idx} * CacheDecode) := 
+      (fun c => Ifopt (nth_opt v idx) as b
+                Then Some (b, existT _ (S idx) eq_refl, addD c 8) Else None).
+
+  (* This can be made much better but I wanted to make sure I knew how to write this 
+     program since it uses fix with a measure *)
+  Lemma mr :
+    forall n idx,
+      Nat.leb n idx = false -> 
+      MR lt (fun idx'0 : nat => n - idx'0) (S idx) idx.
+  Proof.
+    red; auto.
+  Qed.
+
+  Definition consume_bytes {m} (num : nat) (buf : ByteBuffer.t m) idx cd :=
+    fold_left (fun (acc : option (nat*CacheDecode)) _ =>
+                 acc' <- acc;
+                 (* next <- GetCurrentByte buf (fst acc') (snd acc'); *)
+                  next <- GetByteAt (fst acc') buf (fst acc') (snd acc');
+                 let '(_, idx', cd') := next in
+                 Some (idx', cd')
+              ) (seq idx num) (Some (idx, cd)).
+
+  Definition bytes_to_string_opt {m} (num : nat) (buf : ByteBuffer.t m) idx cd
+    : option string :=
+    sequence (map (fun elt => option_map (compose fst fst) elt)
+                (map (fun i => GetByteAt i buf idx cd) (seq idx num))).
+
+  Definition AlignedDecodeStringWithTerm' {n}
              (close : string)
-    : AlignedDecodeM string m.
+    : nat -> ByteBuffer.t n -> CacheDecode -> option (string * nat * CacheDecode).
+    refine (Fix (measure_wf Wf_nat.lt_wf (fun idx' => n - idx'))
+         (fun _ => ByteBuffer.t n -> CacheDecode -> option (string * nat * CacheDecode))
+           (fun idx rec buf cd =>
+              (if Nat.leb n idx as eqb return (Nat.leb n idx = eqb -> _) then
+                fun _ => None
+              else
+                fun _ => 
+                term <- bytes_to_string_opt (String.length close) buf idx cd;
+              if term =? close then
+                    (* This should be traverse *)
+                    res <- consume_bytes (String.length close) buf idx cd;
+                Some ("", fst res, snd res)
+                (* Some ("", fst res, snd res) *)
+              else
+                `(b, idx', cd') <- GetCurrentByte buf idx cd;
+                `(s, idx'', cd'') <- rec (S idx) _ buf cd';
+                 Some(String (ascii_of_N (wordToN b)) s, idx'', cd'')
+              ) eq_refl)).
+    apply (mr n idx e).
+    Defined.
+
+  Definition AlignedDecodeStringWithTerm {n} (close : string)
+    : AlignedDecodeM string n :=
+    fun buf idx => AlignedDecodeStringWithTerm' close idx buf.
+  
+  Close Scope option.
+  Ltac unf H := 
+    repeat (
+    unfold DecodeBindOpt2 in H;
+    unfold BindOpt in H;
+    unfold If_Opt_Then_Else in H;
+    unfold DecodeBindOpt in H;
+    unfold Bind2 in H;
+    unfold BindOpt in H).
+
+  Ltac unfg := 
+    repeat (unfold DecodeBindOpt2;
+    unfold BindOpt;
+    unfold If_Opt_Then_Else;
+    unfold DecodeBindOpt;
+    unfold Bind2;
+    unfold BindOpt).
+
+  Lemma option_bind_eq : forall A B (f : A -> option B) o o'
+      (H1 : option_bind f o = option_bind f o')
+      (H : forall x y, f x = f y -> x = y)
+      (H0 : forall x, f x <> None),
+      o = o'.
+  Proof.
+    clear.
+    intros.
+    destruct o,o' eqn:Ho; simpl in *; eauto.
+    {
+      f_equal; eauto.
+    }
+    {
+      exfalso.
+      eapply H0; eauto.
+    }
+    {
+      symmetry in H1.
+      exfalso.
+      eapply H0; eauto.
+    }
+  Qed.
+
+  Require Import BinNums.
+  Require Import BinPos.
+  Require Import BinNat.
+  Lemma lt_n_p : forall (p : positive) (n : N),
+      BinNat.N.lt (BinNums.Npos p) n ->
+      BinPos.Pos.lt p (Pos.of_nat (N.to_nat n)).
+  Proof.
+    clear.
+    intros.
+    lia.
+  Qed.
+
+  Require Import BinNums.
+  Require Import BinPos.
+  Require Import Coq.Strings.Ascii.
+(* Lemma ascii_of_pos_inv : *)
+(*   forall p p',  *)
+(*     ascii_of_pos p = ascii_of_pos p' ->  *)
+(*     (p < 256)%positive -> (p' < 256)%positive ->  *)
+(*     p = p'. *)
+(* Proof. *)
+(*   intros. *)
+(*   unfold ascii_of_pos in H1. *)
+(*   destruct p. *)
+  
+
+  Lemma of_NB : forall n b,
+      Some b = Byte.of_N n -> n = (Byte.to_N b).
+  Proof.
+    clear; simpl; intros.
+    destruct n; simpl in *; auto.
+    inversion H.
+    auto.
+    repeat match goal with
+             | H: context[match ?p with | _ => _ end] |- _ =>
+               destruct p
+             end; inversion H; auto.
+  Qed.
+
+  Lemma ByteOfN_None : forall p, 
+      None = Byte.of_N (N.pos p) ->
+      (Pos.lt 255 p)%positive.
+  Proof.
+    clear.
+    intros.
+    simpl in *.
+    repeat match goal with
+           | H: context[match ?p with | _ => _ end] |- _ =>
+             destruct p
+           end; inversion H; lia.
+  Qed.
+
+  Lemma byte_of_N_inv : forall n n',
+      BinNat.N.lt n 256 -> 
+      BinNat.N.lt n' 256 -> 
+      Byte.of_N n = Byte.of_N n' ->
+      n = n'.
+  Proof.
+    clear.
+    destruct n.
+    {
+      intros.
+      destruct n'; auto.
+      simpl in *.
+      repeat match goal with
+             | H: context[match ?p with | _ => _ end] |- _ =>
+               destruct p
+             end; try inversion H1; lia.
+    }
+    {
+      intros.
+      destruct n'; auto.
+      {
+        simpl in *.
+        repeat match goal with
+             | H: context[match ?p with | _ => _ end] |- _ =>
+               destruct p
+             end; try inversion H1; lia.
+      }        
+      {
+        simpl Byte.of_N at 1 in H1.
+        repeat match goal with
+               | H: context[match ?p with | _ => _ end = _] |- _ =>
+                 destruct p
+               end;
+          match goal with
+          | H: Some ?b = Byte.of_N _ |- _ =>
+            apply of_NB in H1; subst; auto
+          | H : None = Byte.of_N _ |- _ =>
+            apply ByteOfN_None in H; lia
+          end.
+      }
+    }
+  Qed.
+
+  Lemma ascii_of_byte_helper : forall a b,
+      a = ascii_of_byte b -> b = (byte_of_ascii a).
+  Proof.
+    clear.
+    intros.
+    destruct b; subst; auto.
+  Qed.
+
+  Lemma ascii_of_Byte_inv : forall b b',
+      ascii_of_byte b = ascii_of_byte b' ->
+      b = b'.
+  Proof.
+    clear.
+    intros.
+    unfold ascii_of_byte at 1 in H.
+    destruct b;
+    simpl in *;
+    apply ascii_of_byte_helper in H; subst;
+    auto.
+  Qed.
+
+  Definition pos_of_ascii (a : ascii) : positive :=
+    Pos.of_nat (nat_of_ascii a).
+
+  Lemma ascii_of_pos_eq : forall a p, 
+      (p < 256)%positive ->
+      a = ascii_of_pos p ->
+      p = pos_of_ascii a.
+  Proof.
+    clear; intros.
+    unfold ascii_of_pos in H0.
+    repeat match goal with
+             | H: context[match ?p with | _ => _ end] |- _ =>
+               destruct p; try (simpl in *; subst; auto; lia)
+             end.
+  Qed.
+
+  Lemma ascii_of_N_inv : forall n n',
+      BinNat.N.lt n 256 -> 
+      BinNat.N.lt n' 256 -> 
+      ascii_of_N n = ascii_of_N n' ->
+      n = n'.
+  Proof.
+    clear.
+    intros.
+    destruct n; intros;
+    simpl in *.
+    {
+      destruct n'; auto.
+      unfold ascii_of_N in H1.
+      assert (zero = Ascii false false false false false false false false) by auto.
+      assert (one = Ascii true false false false false false false false) by auto.
+      eauto.
+      unfold ascii_of_pos in H1.
+      destruct p.
+      -
+        repeat match goal with
+        | H: context[match ?p with | _ => _ end] |- _ =>
+          destruct p
+        end; inversion H1.
+      -
+        repeat match goal with
+        | H: context[match ?p with | _ => _ end] |- _ =>
+          destruct p
+        end; inversion H1.
+        simpl in *.
+        exfalso.
+        {
+          clear -H0.
+          destruct p; 
+          inversion H0.
+        }
+      -
+        inversion H1.
+    }
+    {
+      destruct n'; auto.
+      unfold ascii_of_N in H1.
+      assert (zero = Ascii false false false false false false false false) by auto.
+      assert (one = Ascii true false false false false false false false) by auto.
+      eauto.
+      unfold ascii_of_pos in H1.
+      destruct p.
+      -
+        repeat match goal with
+        | H: context[match ?p with | _ => _ end] |- _ =>
+          destruct p
+        end; inversion H1.
+      -
+        repeat match goal with
+        | H: context[match ?p with | _ => _ end] |- _ =>
+          destruct p
+        end; inversion H1.
+        simpl in *.
+        exfalso.
+        {
+          clear -H.
+          destruct p; 
+          inversion H.
+        }
+      -
+        inversion H1.
+      -
+        simpl in *.
+        f_equal.
+        assert ((p < 256)%positive) by lia.
+        assert ((p0 < 256)%positive) by lia.
+        clear H H0.
+        unfold ascii_of_pos at 1 in H1.
+        repeat match goal with
+               | H: context[match ?p with | _ => _ end] |- _ =>
+                 destruct p
+               end;
+        apply ascii_of_pos_eq in H1;
+        subst; auto; lia.
+    }
+  Qed.
+
+  Lemma ascii_word_inj : forall (c c0 : word 8),
+      ascii_of_N (wordToN c) = ascii_of_N (wordToN c0) ->
+      c = c0.
+  Proof.
+    clear.
+    intros.
+    apply ascii_of_N_inv in H; eauto.
+    apply wordToN_inj; auto.
+    apply (InternetChecksum.wordToN_bound c).
+    apply (InternetChecksum.wordToN_bound c0).
+  Qed.
+
+  Lemma sequence_eq : forall l l',
+      (forall e, In e l -> e <> None) -> 
+      (forall e, In e l' -> e <> None) -> 
+      sequence l = sequence l' ->
+      l = l'.
+  Proof.
+    clear.
+    induction l.
+    {
+      intros l' H1 H2 H.
+      simpl in *.
+      destruct l'; auto.
+      destruct o.
+      simpl in H.
+      unfold option_bind in H1.
+      destruct (sequence l'); simpl in *; try inversion H.
+      simpl in H.
+      inversion H.
+    }
+    {
+      intros l' H1 H2 H.
+      destruct l'.
+      {
+        destruct a.
+        simpl in *.
+        destruct (sequence l);
+          simpl in *;
+          inversion H.
+        simpl in *.
+        inversion H.
+      }
+      assert (sequence l = sequence l').
+      {
+        unfold option_bind in H.
+        simpl in H.
+        destruct a,o.
+        -
+          destruct (sequence l), (sequence l'); auto;
+            inversion H.
+          apply ascii_of_N_inv in H3; auto.
+          apply (InternetChecksum.wordToN_bound c).
+          apply (InternetChecksum.wordToN_bound c0).
+        -
+          specialize (H2 None).
+          exfalso.
+          apply H2; intuition; auto.
+        -
+          specialize (H1 None).
+          exfalso.
+          apply H1; intuition; auto.
+        -
+          specialize (H1 None).
+          exfalso.
+          apply H1; intuition; auto.
+      }
+      {
+        apply IHl in H0; auto.
+        {
+          subst.
+          clear IHl.
+          simpl in H.
+          apply option_bind_eq in H; subst; auto.
+          intros.
+          {
+            destruct ((sequence l')) eqn:Hl.
+            {
+              simpl in *.
+              inversion H0; subst; auto using ascii_of_N_inv.
+              apply ascii_of_N_inv in H4; auto.
+              apply wordToN_inj in H4; auto.
+              apply (InternetChecksum.wordToN_bound x).
+              apply (InternetChecksum.wordToN_bound y).
+            }
+            {
+              simpl in *.
+              exfalso.
+              assert (forall e, In e l' -> e <> None).
+              {
+                intros; intuition.
+                subst; auto.
+                eapply H2; eauto.
+              }
+              clear -Hl H3.
+              induction l'; inversion Hl.
+              destruct a.
+              2:{
+                simpl in *.
+                eapply H3; intuition; subst; eauto.
+              }
+              {
+                simpl in Hl.
+                destruct ((sequence l')).
+                simpl in *.
+                inversion Hl.
+                simpl in *.
+                apply IHl'; auto.
+              }
+            }
+          }
+          {
+            intros.
+            intuition.
+            assert (forall e, In e l' -> e <> None).
+            {
+              intros; intuition.
+              subst; auto.
+              eapply H2; eauto.
+              simpl in *.
+              right; auto.
+            }
+            clear -H0 H3.
+            induction l'.
+            simpl in *.
+            inversion H0.
+            destruct a.
+            simpl in *.
+            destruct ((sequence l')).
+            simpl in *.
+            inversion H0.
+            simpl in *.
+            eauto.
+            simpl in *.
+            eapply H3; intuition; subst; auto.
+          }
+        }
+        {
+          intuition; eauto.
+          subst; auto.
+          eapply H1; eauto.
+          right; auto.
+        }
+        {
+          intuition; eauto.
+          subst; auto.
+          eapply H2; eauto.
+          right; auto.
+        }
+      }
+    }
+  Qed.
+
+  Lemma getByteNot_None : forall n (buf : ByteBuffer.t n) idx cd e,
+      In e (map (fun i => GetByteAt i buf idx cd) (seq 0 n)) ->
+      e <> None.
+  Proof.
+    clear; intros.
+    induction n.
+    simpl in *.
+    inversion H.
+    simpl in *.
+    destruct H; subst; intuition; eauto.
+    {
+      destruct n.
+      simpl in *.
+      unfold GetByteAt in H.
+      destruct (nth_opt buf 0) eqn:He; inversion H.
+      simpl in *.
+      unfold nth_opt in He.      
+      simpl in *.
+      clear -He.      
+      (* assert (buf <> @Vector.nil Core.char). *)
+      (* destruct buf; auto. *)
+      (* simpl in *. *)
+      admit.
+      admit.
+    }
   Admitted.
+
+  Lemma asdf : forall A B C O (f : option (A*B*C) -> option O)
+                      (l l' : list (option (A*B*C))),
+      (forall (a b: option (A*B*C)),
+          f a = f b -> option_map (compose fst fst) a = option_map (compose fst  fst) b) ->
+      map f l = map f l' ->
+      map (option_map (compose fst fst)) l = map (option_map (compose fst fst)) l'.
+  Proof.
+    clear.
+    induction l; simpl; intros.
+    {
+      symmetry in H0.
+      apply map_eq_nil in H0.
+      subst; auto.
+    }
+    {
+      destruct l'.      
+      simpl in *.
+      discriminate.
+      simpl in H0.
+      inversion H0; auto.
+      apply H in H2.
+      simpl.
+      rewrite H2.
+      f_equal.      
+      apply IHl; auto.
+    }
+  Qed.
+
+  (* Require Import CoLoR.Util.Vector.VecUtil. *)
+  Lemma nth_opt_cons : forall T (h : T) m (v : Vector.t T m) a,
+      Vector_nth_opt (Vector.cons T h m v) (S a) =
+      Vector_nth_opt v a.
+  Proof.
+    clear.
+    destruct v; simpl; auto.
+  Qed.
+
+  Lemma getByteAt_fst_fst_tl : 
+    forall a (m : nat) (v : ByteBuffer.t (S m)) (n : nat) (cd : CacheDecode),
+      option_map (fst ∘ fst) (GetByteAt a (Vector.tl v) n cd) =
+      option_map (fst ∘ fst) (GetByteAt (S a) v (S n) cd).
+  Proof.
+    clear.
+    intros.
+    unfold GetByteAt.
+    dependent destruction v.
+    simpl.
+    unfold nth_opt.
+    rewrite nth_opt_cons.
+    destruct Vector_nth_opt; simpl; auto.
+  Qed.
+
+  Lemma bytes_to_string_eq : forall m num (v : ByteBuffer.t (S m)) n cd, 
+        bytes_to_string_opt num (Vector.tl v) n cd =
+        bytes_to_string_opt num v (S n) cd.
+  Proof.
+    clear.
+    intros.
+    unfold bytes_to_string_opt.
+    rewrite <- seq_shift.
+    induction (seq n num); simpl; auto.
+    simpl.
+    rewrite IHl.
+    rewrite getByteAt_fst_fst_tl.
+    auto.
+  Qed.
+    
+  Lemma foldl_cons : forall A B (f : A -> B -> A) l (elt : B) (acc : A),
+      fold_left f l (f acc elt) = f (fold_left f l acc) elt .
+  Proof.
+    clear.
+    induction l; auto.
+    intros.
+  Admitted.
+    
+    
+  Lemma getByteAt_snd_fst_tl : 
+    forall a (m : nat) (v : ByteBuffer.t (S m)) (n : nat) (cd : CacheDecode),
+      option_map (compose S (snd ∘ fst)) (GetByteAt a (Vector.tl v) n cd) =
+      option_map (snd ∘ fst) (GetByteAt (S a) v (S n) cd).
+  Proof.
+    clear.
+    intros.
+    unfold GetByteAt.
+    dependent destruction v.
+    simpl.
+    unfold nth_opt.
+    rewrite nth_opt_cons.
+    destruct Vector_nth_opt; simpl; auto.
+  Qed.
+
+  Lemma getByteAt_snd_tl : 
+    forall a (m : nat) (v : ByteBuffer.t (S m)) (n : nat) (cd : CacheDecode),
+      option_map snd (GetByteAt a (Vector.tl v) n cd) =
+      option_map snd (GetByteAt (S a) v (S n) cd).
+  Proof.
+    clear.
+    intros.
+    unfold GetByteAt.
+    dependent destruction v.
+    simpl.
+    unfold nth_opt.
+    rewrite nth_opt_cons.
+    destruct Vector_nth_opt; simpl; auto.
+  Qed.
+    
+  Lemma comsume_bytes_snd_eq :
+    forall (m n num : nat) (v : Vector.t Core.char (S m))
+           (cd : CacheDecode),
+      option_map snd (consume_bytes num (Vector.tl v) n cd) = 
+      option_map snd (consume_bytes num v (S n) cd).
+  Proof.
+    clear.
+    intros.
+    unfold consume_bytes.
+    rewrite <- seq_shift.
+    assert (option_map (compose S fst) (Some (n, cd)) =
+            option_map fst (Some (S n, cd))).
+    auto.
+    assert (option_map snd (Some (n, cd)) =
+            option_map snd (Some (S n, cd))).
+    auto.
+    (* rewrite <- ListFacts.fold_map. *)
+    generalize dependent (Some (S n, cd)).
+    generalize dependent (Some (n, cd)).
+    generalize dependent m.
+    generalize dependent cd.
+    induction (seq n num); simpl; auto.
+    intros.
+    assert (option_map snd (option_bind (fun '(_, idx', cd') => Some (idx', cd'))
+                          (GetByteAt n (Vector.tl v) n cd)) =
+            (option_map snd (option_bind (fun '(_, idx', cd') => Some (idx', cd'))
+          (GetByteAt (S n) v (S n) cd)))).
+    {
+      clear.
+      unfold GetByteAt.
+      dependent destruction v.
+      simpl.
+      unfold nth_opt.
+      rewrite nth_opt_cons.
+      destruct Vector_nth_opt; simpl; auto.
+    }
+    assert (option_map (compose S fst)
+                       (option_bind (fun '(_, idx', cd') => Some (idx', cd'))
+                          (GetByteAt n (Vector.tl v) n cd)) =
+            (option_map fst (option_bind (fun '(_, idx', cd') => Some (idx', cd'))
+          (GetByteAt (S n) v (S n) cd)))).
+    {
+      clear.
+      unfold GetByteAt.
+      dependent destruction v.
+      simpl.
+      unfold nth_opt.
+      rewrite nth_opt_cons.
+      destruct Vector_nth_opt; simpl; auto.
+    }
+    rewrite IHl with (o := (option_bind
+          (fun acc' : nat * CacheDecode =>
+           option_bind (fun '(_, idx', cd') => Some (idx', cd'))
+             (GetByteAt (fst acc') (Vector.tl v) (fst acc') (snd acc'))) o))
+    (o0 := (option_bind
+          (fun acc' : nat * CacheDecode =>
+           option_bind (fun '(_, idx', cd') => Some (idx', cd'))
+             (GetByteAt (fst acc') v (fst acc') (snd acc'))) o0)); auto.
+    {
+      unfold option_map.
+      unfold option_bind.
+      clear -H H2 H0.
+      destruct o,o0; auto;
+        destruct_conjs;
+        simpl in *;
+        unfold compose in *;
+        simpl in *;
+        inversion H;
+        subst;
+        inversion H0; subst;
+        clear H H0.
+        destruct (GetByteAt n1 (Vector.tl v) n1 c) eqn:Ht;
+          destruct (GetByteAt (S n1) v (S n1) c) eqn:Hv;
+          destruct_conjs; simpl in *;
+            auto;
+            match goal with
+            | H1: context[GetByteAt ?n1 (Vector.tl ?v) ?n1 ?c],
+              H2: context[GetByteAt (S ?n1) ?v (S ?n1) ?c]
+              |- _ =>
+              assert (H3: option_map (S ∘ (snd ∘ fst)) (GetByteAt n1 (Vector.tl v) n1 c) =
+                      option_map (snd ∘ fst) (GetByteAt (S n1) v (S n1) c)) by
+                  apply getByteAt_snd_fst_tl;
+              rewrite H1 in H3; rewrite H2 in H3;
+              inversion H3; subst; auto
+            end.
+    }
+    {
+      unfold option_map.
+      unfold option_bind.
+      destruct o,o0; auto;
+      destruct_conjs;
+        simpl in *;
+        unfold compose in *;
+        simpl in *;
+      inversion H; inversion H0; subst;
+      clear H H0;
+      destruct (GetByteAt n1 (Vector.tl v) n1 c) eqn:Ht;
+        destruct (GetByteAt (S n1) v (S n1) c) eqn:Hv;
+          destruct_conjs; simpl in *; auto;
+      match goal with
+      | H1: context[GetByteAt ?n1 (Vector.tl ?v) ?n1 ?c],
+            H2: context[GetByteAt (S ?n1) ?v (S ?n1) ?c]
+        |- _ =>
+        assert (H3: option_map snd (GetByteAt n1 (Vector.tl v) n1 c) =
+                    option_map snd (GetByteAt (S n1) v (S n1) c))
+          by
+            apply getByteAt_snd_tl;
+        rewrite H1 in H3; rewrite H2 in H3;
+        inversion H3; subst; auto
+      end.
+    }
+  Qed.
+
+  Lemma comsume_bytes_fst_eq :
+    forall (m n num : nat) (v : Vector.t Core.char (S m))
+           (cd : CacheDecode),
+      option_map (compose S fst) (consume_bytes num (Vector.tl v) n cd) = 
+      option_map fst (consume_bytes num v (S n) cd).
+  Proof.
+    clear.
+    intros.
+    unfold consume_bytes.
+    rewrite <- seq_shift.
+    assert (option_map (compose S fst) (Some (n, cd)) =
+            option_map fst (Some (S n, cd))).
+    auto.
+    assert (option_map snd (Some (n, cd)) =
+            option_map snd (Some (S n, cd))).
+    auto.
+    generalize dependent (Some (S n, cd)).
+    generalize dependent (Some (n, cd)).
+    generalize dependent m.
+    generalize dependent cd.
+    induction (seq n num); simpl; auto.
+    intros.
+    assert (option_map snd (option_bind (fun '(_, idx', cd') => Some (idx', cd'))
+                          (GetByteAt n (Vector.tl v) n cd)) =
+            (option_map snd (option_bind (fun '(_, idx', cd') => Some (idx', cd'))
+          (GetByteAt (S n) v (S n) cd)))).
+    {
+      clear.
+      unfold GetByteAt.
+      dependent destruction v.
+      simpl.
+      unfold nth_opt.
+      rewrite nth_opt_cons.
+      destruct Vector_nth_opt; simpl; auto.
+    }
+    assert (option_map (compose S fst)
+                       (option_bind (fun '(_, idx', cd') => Some (idx', cd'))
+                          (GetByteAt n (Vector.tl v) n cd)) =
+            (option_map fst (option_bind (fun '(_, idx', cd') => Some (idx', cd'))
+          (GetByteAt (S n) v (S n) cd)))).
+    {
+      clear.
+      unfold GetByteAt.
+      dependent destruction v.
+      simpl.
+      unfold nth_opt.
+      rewrite nth_opt_cons.
+      destruct Vector_nth_opt; simpl; auto.
+    }
+    rewrite IHl with (o := (option_bind
+          (fun acc' : nat * CacheDecode =>
+           option_bind (fun '(_, idx', cd') => Some (idx', cd'))
+             (GetByteAt (fst acc') (Vector.tl v) (fst acc') (snd acc'))) o))
+    (o0 := (option_bind
+          (fun acc' : nat * CacheDecode =>
+           option_bind (fun '(_, idx', cd') => Some (idx', cd'))
+             (GetByteAt (fst acc') v (fst acc') (snd acc'))) o0)); auto.
+    {
+      unfold option_map.
+      unfold option_bind.
+      clear -H H2 H0.
+      destruct o,o0; auto;
+        destruct_conjs;
+        simpl in *;
+        unfold compose in *;
+        simpl in *;
+        inversion H;
+        subst;
+        inversion H0; subst;
+        clear H H0.
+        destruct (GetByteAt n1 (Vector.tl v) n1 c) eqn:Ht;
+          destruct (GetByteAt (S n1) v (S n1) c) eqn:Hv;
+          destruct_conjs; simpl in *;
+            auto;
+            match goal with
+            | H1: context[GetByteAt ?n1 (Vector.tl ?v) ?n1 ?c],
+              H2: context[GetByteAt (S ?n1) ?v (S ?n1) ?c]
+              |- _ =>
+              assert (H3: option_map (S ∘ (snd ∘ fst)) (GetByteAt n1 (Vector.tl v) n1 c) =
+                      option_map (snd ∘ fst) (GetByteAt (S n1) v (S n1) c)) by
+                  apply getByteAt_snd_fst_tl;
+              rewrite H1 in H3; rewrite H2 in H3;
+              inversion H3; subst; auto
+            end.
+    }
+    {
+      unfold option_map.
+      unfold option_bind.
+      destruct o,o0; auto;
+      destruct_conjs;
+        simpl in *;
+        unfold compose in *;
+        simpl in *;
+      inversion H; inversion H0; subst;
+      clear H H0;
+      destruct (GetByteAt n1 (Vector.tl v) n1 c) eqn:Ht;
+        destruct (GetByteAt (S n1) v (S n1) c) eqn:Hv;
+          destruct_conjs; simpl in *; auto;
+      match goal with
+      | H1: context[GetByteAt ?n1 (Vector.tl ?v) ?n1 ?c],
+            H2: context[GetByteAt (S ?n1) ?v (S ?n1) ?c]
+        |- _ =>
+        assert (H3: option_map snd (GetByteAt n1 (Vector.tl v) n1 c) =
+                    option_map snd (GetByteAt (S n1) v (S n1) c))
+          by
+            apply getByteAt_snd_tl;
+        rewrite H1 in H3; rewrite H2 in H3;
+        inversion H3; subst; auto
+      end.
+    }
+  Qed.
 
   Lemma AlignedDecodeStringWithTermM {C : Type}
         (close : string)
@@ -41,6 +900,306 @@ Section String.
            (fun numBytes => s <- AlignedDecodeStringWithTerm close;
                           t' s).
   Proof.
+    split.
+    {
+      intros.
+      unfold AlignedDecodeStringWithTerm.
+      unfg.
+      unfold BindAlignedDecodeM.
+      unfold AlignedDecodeStringWithTerm'.
+      rewrite Init.Wf.Fix_eq.
+      simpl.
+      destruct (Nat.leb numBytes_hd n) eqn:Hn.
+      assert (Help: (Fix (measure_wf Wf_nat.lt_wf (fun idx' : nat => numBytes_hd - idx'))
+            (constant (ByteBuffer.t numBytes_hd ->
+                       CacheDecode -> option (string * nat * CacheDecode)))
+            (fun (idx : nat)
+               (rec : forall y : nat,
+                      MR lt (fun idx' : nat => numBytes_hd - idx') y idx ->
+                      ByteBuffer.t numBytes_hd ->
+                      CacheDecode -> option (string * nat * CacheDecode))
+               (buf : ByteBuffer.t numBytes_hd) (cd0 : CacheDecode) =>
+             (if Nat.leb numBytes_hd idx as eqb
+               return
+                 (Nat.leb numBytes_hd idx = eqb -> option (string * nat * CacheDecode))
+              then constant None
+              else
+               fun H0 : Nat.leb numBytes_hd idx = false =>
+               option_bind
+                 (fun term : string =>
+                  if term =? close
+                  then
+                   option_bind
+                     (fun res : nat * CacheDecode => Some ("", fst res, snd res))
+                     (consume_bytes (String.length close) buf idx cd0)
+                  else
+                   `(b, _, cd') <- GetCurrentByte buf idx cd0;
+                   `(s, idx'', cd'') <- rec (S idx) (mr numBytes_hd idx H0) buf cd';
+                   Some (String (ascii_of_N (wordToN b)) s, idx'', cd''))
+                 (bytes_to_string_opt (String.length close) buf idx cd0)) eq_refl) n
+            (Vector.tl v) cd) = (
+(if Nat.leb numBytes_hd n as eqb
+      return (Nat.leb numBytes_hd n = eqb -> option (string * nat * CacheDecode))
+     then constant None
+     else
+      constant option_bind
+                 (fun term : string =>
+                  if term =? close
+                  then
+                   option_bind
+                     (fun res : nat * CacheDecode => Some ("", fst res, snd res))
+                     (consume_bytes (String.length close) (Vector.tl v) n cd)
+                  else
+                   `(b0, _, cd') <- GetCurrentByte (Vector.tl v) n cd;
+                   `(s, idx'', cd'') <- Fix
+                                          (measure_wf Wf_nat.lt_wf
+                                             (fun idx' : nat => numBytes_hd - idx'))
+                                          (constant (ByteBuffer.t numBytes_hd ->
+                                                     CacheDecode ->
+                                                     option (string * nat * CacheDecode)))
+                                          (fun (idx : nat)
+                                             (rec : forall y : nat,
+                                                    MR lt
+                                                      (fun idx' : nat =>
+                                                       numBytes_hd - idx') y idx ->
+                                                    ByteBuffer.t numBytes_hd ->
+                                                    CacheDecode ->
+                                                    option (string * nat * CacheDecode))
+                                             (buf : ByteBuffer.t numBytes_hd)
+                                             (cd0 : CacheDecode) =>
+                                           (if Nat.leb numBytes_hd idx as eqb
+                                             return
+                                               (Nat.leb numBytes_hd idx = eqb ->
+                                                option (string * nat * CacheDecode))
+                                            then constant None
+                                            else
+                                             fun H1 : Nat.leb numBytes_hd idx = false =>
+                                             option_bind
+                                               (fun term0 : string =>
+                                                if term0 =? close
+                                                then
+                                                 option_bind
+                                                   (fun res : nat * CacheDecode =>
+                                                    Some ("", fst res, snd res))
+                                                   (consume_bytes 
+                                                      (String.length close) buf idx cd0)
+                                                else
+                                                 `(b1, _, cd'0) <- 
+                                                 GetCurrentByte buf idx cd0;
+                                                 `(s, idx'', cd'') <- 
+                                                 rec (S idx) 
+                                                   (mr numBytes_hd idx H1) buf cd'0;
+                                                 Some
+                                                   (String (ascii_of_N (wordToN b1)) s,
+                                                   idx'', cd''))
+                                               (bytes_to_string_opt
+                                                  (String.length close) buf idx cd0))
+                                             eq_refl) (S n) 
+                                          (Vector.tl v) cd';
+                   Some (String (ascii_of_N (wordToN b0)) s, idx'', cd''))
+                 (bytes_to_string_opt (String.length close) (Vector.tl v) n cd)) eq_refl
+                          )
+    ).
+        rewrite Init.Wf.Fix_eq.
+        auto.
+        admit.
+        rewrite Help.
+      {
+        rewrite Hn; auto.
+      }
+      {
+        assert (ahh: Fix (measure_wf Wf_nat.lt_wf (fun idx' : nat => numBytes_hd - idx'))
+            (constant (ByteBuffer.t numBytes_hd ->
+                       CacheDecode -> option (string * nat * CacheDecode)))
+            (fun (idx : nat)
+               (rec : forall y : nat,
+                      MR lt (fun idx' : nat => numBytes_hd - idx') y idx ->
+                      ByteBuffer.t numBytes_hd ->
+                      CacheDecode -> option (string * nat * CacheDecode))
+               (buf : ByteBuffer.t numBytes_hd) (cd0 : CacheDecode) =>
+             (if Nat.leb numBytes_hd idx as eqb
+               return
+                 (Nat.leb numBytes_hd idx = eqb -> option (string * nat * CacheDecode))
+              then constant None
+              else
+               fun H0 : Nat.leb numBytes_hd idx = false =>
+               option_bind
+                 (fun term : string =>
+                  if term =? close
+                  then
+                   option_bind
+                     (fun res : nat * CacheDecode => Some ("", fst res, snd res))
+                     (consume_bytes (String.length close) buf idx cd0)
+                  else
+                   `(b, _, cd') <- GetCurrentByte buf idx cd0;
+                   `(s, idx'', cd'') <- rec (S idx) (mr numBytes_hd idx H0) buf cd';
+                   Some (String (ascii_of_N (wordToN b)) s, idx'', cd''))
+                 (bytes_to_string_opt (String.length close) buf idx cd0)) eq_refl) n
+            (Vector.tl v) cd =
+                ((if Nat.leb numBytes_hd n as eqb
+      return (Nat.leb numBytes_hd n = eqb -> option (string * nat * CacheDecode))
+     then constant None
+     else
+      constant option_bind
+                 (fun term : string =>
+                  if term =? close
+                  then
+                   option_bind
+                     (fun res : nat * CacheDecode => Some ("", fst res, snd res))
+                     (consume_bytes (String.length close) (Vector.tl v) n cd)
+                  else
+                   `(b0, _, cd') <- GetCurrentByte (Vector.tl v) n cd;
+                   `(s, idx'', cd'') <- Fix
+                                          (measure_wf Wf_nat.lt_wf
+                                             (fun idx' : nat => numBytes_hd - idx'))
+                                          (constant (ByteBuffer.t numBytes_hd ->
+                                                     CacheDecode ->
+                                                     option (string * nat * CacheDecode)))
+                                          (fun (idx : nat)
+                                             (rec : forall y : nat,
+                                                    MR lt
+                                                      (fun idx' : nat =>
+                                                       numBytes_hd - idx') y idx ->
+                                                    ByteBuffer.t numBytes_hd ->
+                                                    CacheDecode ->
+                                                    option (string * nat * CacheDecode))
+                                             (buf : ByteBuffer.t numBytes_hd)
+                                             (cd0 : CacheDecode) =>
+                                           (if Nat.leb numBytes_hd idx as eqb
+                                             return
+                                               (Nat.leb numBytes_hd idx = eqb ->
+                                                option (string * nat * CacheDecode))
+                                            then constant None
+                                            else
+                                             fun H1 : Nat.leb numBytes_hd idx = false =>
+                                             option_bind
+                                               (fun term0 : string =>
+                                                if term0 =? close
+                                                then
+                                                 option_bind
+                                                   (fun res : nat * CacheDecode =>
+                                                    Some ("", fst res, snd res))
+                                                   (consume_bytes 
+                                                      (String.length close) buf idx cd0)
+                                                else
+                                                 `(b1, _, cd'0) <- 
+                                                 GetCurrentByte buf idx cd0;
+                                                 `(s, idx'', cd'') <- 
+                                                 rec (S idx) 
+                                                   (mr numBytes_hd idx H1) buf cd'0;
+                                                 Some
+                                                   (String (ascii_of_N (wordToN b1)) s,
+                                                   idx'', cd''))
+                                               (bytes_to_string_opt
+                                                  (String.length close) buf idx cd0))
+                                             eq_refl) (S n) 
+                                          (Vector.tl v) cd';
+                   Some (String (ascii_of_N (wordToN b0)) s, idx'', cd''))
+                 (bytes_to_string_opt (String.length close) (Vector.tl v) n cd))) eq_refl).
+        {
+          rewrite Init.Wf.Fix_eq.
+          admit.
+          admit.
+        }
+        rewrite ahh.
+        simpl.
+        clear ahh.
+        rewrite Hn; auto.
+        unfold option_bind.
+        rewrite bytes_to_string_eq.
+        destruct (bytes_to_string_opt (String.length close) v (S n) cd); simpl; auto.
+        destruct (s =? close)%string.
+        -
+          destruct (consume_bytes (String.length close) v (S n) cd) eqn:Hv.
+          {
+            destruct (consume_bytes (String.length close) (Vector.tl v) n cd) eqn:Ht.
+            {
+              simpl.
+              assert (option_map (compose S fst) (consume_bytes (String.length close) (Vector.tl v) n cd) = option_map fst (consume_bytes (String.length close) v (S n) cd))
+                   by (apply comsume_bytes_fst_eq).
+              rewrite Hv in H0.
+              rewrite Ht in H0.
+              simpl in H0.
+              inversion H0.
+              unfold compose.
+              specialize (H "").
+              destruct H.
+              rewrite H.
+              assert ((option_map snd (consume_bytes (String.length close) (Vector.tl v) n cd) = option_map snd (consume_bytes (String.length close) v (S n) cd)))
+                     by apply comsume_bytes_snd_eq.
+              rewrite Hv in H3.
+              rewrite Ht in H3.
+              simpl in H3.
+              inversion H3; subst; auto.
+            }
+            {
+              exfalso.
+              assert (option_map (compose S fst) (consume_bytes (String.length close) (Vector.tl v) n cd) = option_map fst (consume_bytes (String.length close) v (S n) cd))
+                   by (apply comsume_bytes_fst_eq).
+              rewrite Ht in H0.
+              rewrite Hv in H0.
+              simpl in H0.
+              inversion H0.
+            }
+          }
+          {
+            simpl.
+            destruct (consume_bytes (String.length close)
+                                    (Vector.tl v) n cd) eqn:Ht; auto.
+            exfalso.
+            assert (option_map (compose S fst) (consume_bytes (String.length close) (Vector.tl v) n cd) = option_map fst (consume_bytes (String.length close) v (S n) cd))
+                   by (apply comsume_bytes_fst_eq).
+            rewrite Ht in H0.
+            rewrite Hv in H0.
+            simpl in H0.
+            inversion H0.
+          }
+        -
+          admit.
+      }
+      {
+        intros.
+        repeat (apply functional_extensionality; intros; f_equal).
+        destruct GetCurrentByte; auto;
+          destruct_conjs.
+        assert (f_eq_g : forall y, f y = g y).
+        intros.
+        apply functional_extensionality; intros; f_equal.
+        rewrite f_eq_g.
+        eauto.
+      }
+    }
+      {
+        intros.
+        split
+        repeat (apply functional_extensionality; intros; f_equal).
+        destruct GetCurrentByte; auto;
+          destruct_conjs.
+        assert (f_eq_g : forall y, f y = g y).
+        intros.
+        apply functional_extensionality; intros; f_equal.
+        rewrite f_eq_g.
+        eauto.
+
+      {
+        rewrite Init.Wf.Fix_eq.
+        rewrite Init.Wf.Fix_eq.
+        rewrite Init.Wf.Fix_eq.
+        admit.
+      }
+      {
+        intros.
+        repeat (apply functional_extensionality; intros; f_equal).
+        destruct GetCurrentByte; auto;
+          destruct_conjs.
+        assert (f_eq_g : forall y, f y = g y).
+        intros.
+        apply functional_extensionality; intros; f_equal.
+        rewrite f_eq_g.
+        eauto.
+      }
+    }
+    
   Admitted.
 
 End String.
